atgt/Discont/Limit.lean
@@ -1,5 +1,8 @@
 import atgt.Funcoid
+import atgt.Filtrator.Powerset
+import atgt.Filtrator
 
 universe u v w
 
--- def IsFuncoidLimit {α: Type u} {β: Type v} (d: Funcoid α β) :=
+def IsFuncoidLimit {α: Type u} {β: Type v} (d: Funcoid α β) (F: Filtrator.FilterOnPowerset β) (x: α) :=
+  F ≤ Funcoid.fwd_set d ({x} : Set α)
